Graphlib/SearchCommon.lean
@@ -1,0 +1,354 @@
+import Mathlib.Data.Bool.AllAny
+import Mathlib.Data.FinEnum
+import Mathlib.Data.Finset.Empty
+import Mathlib.Data.List.MinMax
+
+import Graphlib.Lists
+import Graphlib.FinEnum
+import Graphlib.Basic
+
+set_option trace.split.failure true
+--set_option diagnostics true
+
+-- def local global variable for a graph
+--variable {V : Type} {E : Type} [FinEnum V] [DecidableEq V] [DecidableEq E]
+--variable (G : WeightedDiGraph V E)
+
+
+
+-----------------------------------------------------------------------
+------ Search state of the DFS and its invariants
+structure base_search_state [FinEnum V] [DecidableEq E] [DecidableEq V]
+    (g: WeightedDiGraph V E) (start : V) where
+    visited : Finset V
+    pathOrder : V → Nat 
+    mother : visited → V
+    mother_proof (v : visited): ↑v ≠ start → g.Adj (mother v) v
+    stack : List V
+    terminated : Bool
+
+class has_base_search_state [FinEnum V] [DecidableEq E] [DecidableEq V]
+    (g: WeightedDiGraph V E) (start : V) (B : Type) where
+  to_base_state : B → base_search_state g start
+
+
+instance [FinEnum V] [DecidableEq E] [DecidableEq V](g: WeightedDiGraph V E) (start : V):
+    has_base_search_state g start (base_search_state g start) where
+  to_base_state := fun x => x 
+
+
+abbrev search_invar_stack_is_visited [FinEnum V] [DecidableEq E] [DecidableEq V]
+    (g: WeightedDiGraph V E) (start : V) (s : base_search_state g start):=
+      ∀ x : V, x ∈ s.stack → x ∈ s.visited
+
+abbrev search_invar_mother_is_visited [FinEnum V] [DecidableEq E] [DecidableEq V]
+    (g: WeightedDiGraph V E) (start : V) (s : base_search_state g start):=
+      ∀ x : s.visited, s.mother x ∈ s.visited
+
+abbrev search_invar_mother_decreasing_path_order [FinEnum V] [DecidableEq E] [DecidableEq V]
+    (g: WeightedDiGraph V E) (start : V) (s : base_search_state g start) :=
+      ∀ x : s.visited, ↑x ≠ start → s.pathOrder (s.mother x) < s.pathOrder x 
+
+abbrev search_invar_on_stack_or_all_neighbours_visited [FinEnum V] [DecidableEq E] [DecidableEq V]
+    (g: WeightedDiGraph V E) (start : V) (s : base_search_state g start):=
+      ∀ x : s.visited, ↑x ∈ s.stack ∨ ∀ y : V, (g.Adj x y) → y ∈ s.visited
+
+abbrev search_invar_start_visited [FinEnum V] [DecidableEq E] [DecidableEq V]
+    (g: WeightedDiGraph V E) (start : V) (s : base_search_state g start) :=
+      start ∈ s.visited
+
+abbrev search_invar_all_basic[FinEnum V] [DecidableEq E] [DecidableEq V]
+    (g: WeightedDiGraph V E) (start : V) (s : base_search_state g start) :=
+      search_invar_stack_is_visited g start s
+      ∧ search_invar_mother_is_visited g start s
+      ∧ search_invar_mother_decreasing_path_order g start s
+      ∧ search_invar_on_stack_or_all_neighbours_visited g start s
+      ∧ search_invar_start_visited g start s
+
+
+def extract_path_to [FinEnum V] [DecidableEq E] [DecidableEq V]
+    (g: WeightedDiGraph V E) (start : V) (goal : V) (search_state : base_search_state g start)
+    (goal_reached : goal ∈ search_state.visited)
+    (mother_invar : search_invar_mother_is_visited g start search_state)
+    (decreasing_invar : search_invar_mother_decreasing_path_order g start search_state):
+      Σ' (p : Path g start goal), (∀ v ∈ support g p.walk, search_state.pathOrder v ≤ search_state.pathOrder goal):= 
+      if start_is_goal : goal = start then
+        let emptyW : Walk g start goal := start_is_goal ▸ Walk.nil
+        let emptyP : Path g start goal := Path.mk emptyW (by
+          simp [emptyW]
+          unfold support
+          split
+          · next u u' x w rest u_adj_v walk_is_cons => 
+            simp_all
+            subst start_is_goal
+            simp_all only [reduceCtorEq] 
+          · simp
+        )
+
+        have order : ∀ v ∈ support g emptyP.walk, search_state.pathOrder v ≤ search_state.pathOrder goal := by
+          intro a a_in_support
+          unfold emptyP at a_in_support
+          unfold emptyW at a_in_support
+          unfold support at a_in_support
+          simp_all
+          subst start_is_goal
+          simp_all only [List.mem_cons, List.not_mem_nil, or_false, le_refl]
+
+        ⟨ emptyP, order ⟩ 
+      else
+        let goal_predecessor : V := search_state.mother ⟨ goal, goal_reached ⟩
+        let ⟨ path_start_pre, order_proof ⟩ := -- : Path g start goal_predecessor :=
+          extract_path_to g start goal_predecessor search_state (by apply mother_invar) mother_invar decreasing_invar 
+        let pre_adj_goal : g.Adj goal_predecessor goal := search_state.mother_proof ⟨ goal , goal_reached ⟩ start_is_goal
+        let goal_not_visited : goal ∉ support g path_start_pre.walk := by
+          by_contra goal_is_in_support
+          have h := order_proof goal goal_is_in_support
+          unfold goal_predecessor at h
+          unfold search_invar_mother_decreasing_path_order at decreasing_invar
+          have h' := decreasing_invar ⟨ goal, goal_reached⟩ 
+          clear mother_invar decreasing_invar
+          simp_all
+          omega
+
+        let goal_path : Path g start goal := extend_path g path_start_pre pre_adj_goal goal_not_visited
+
+        let new_order_proof : ∀ v ∈ support g goal_path.walk, search_state.pathOrder v ≤ search_state.pathOrder goal := by
+          intro a a_in_support
+          unfold goal_path at a_in_support
+          rw [extend_path_extends_support] at a_in_support
+          simp_all
+          apply a_in_support.elim
+          · intro a_in_old_path
+            apply le_trans 
+            · apply order_proof
+              exact a_in_old_path
+            · unfold goal_predecessor
+              apply le_of_lt
+              exact decreasing_invar ⟨ goal,goal_reached ⟩ start_is_goal
+          · simp_all
+
+        ⟨ goal_path, new_order_proof ⟩ 
+
+termination_by search_state.pathOrder goal
+decreasing_by
+  simp_all only [Subtype.forall, ne_eq, not_false_eq_true]
+
+
+
+
+abbrev search_step_function [FinEnum V] [DecidableEq E] [DecidableEq V]
+    (g: WeightedDiGraph V E) (start : V)
+    {state_type : Type} [has_base_search_state g start state_type] :=
+      V → state_type → state_type × (Option Bool)
+
+
+abbrev search_state_not_terminated [FinEnum V] [DecidableEq E] [DecidableEq V]
+    (g: WeightedDiGraph V E) (start : V) 
+    {state_type : Type} [has_base_search_state g start state_type]
+    (state : state_type):=
+    let base_state : base_search_state g start := (has_base_search_state.to_base_state state)
+    base_state.terminated = false
+
+
+abbrev search_step_does_not_terminate [FinEnum V] [DecidableEq E] [DecidableEq V]
+    (g: WeightedDiGraph V E) (start : V) (goal : V)
+    {state_type : Type} [has_base_search_state g start state_type]
+    (search_step : search_step_function (state_type := state_type) g start) :=
+    ∀ s :
+      state_type,
+        let res : state_type × (Option Bool) := search_step goal s
+        let res_state : base_search_state g start := (has_base_search_state.to_base_state res.fst)
+        res.snd = none → res_state.terminated = false
+
+
+------------------------------------------------------------------------------------------
+-- Search Recurse
+------------------
+def search_recurse [FinEnum V] [DecidableEq E] [DecidableEq V]
+    (g: WeightedDiGraph V E) (start : V)
+    {state_type : Type} [has_base_search_state g start state_type]
+    (goal : V)
+    (priorState : state_type)
+    (not_terminated : search_state_not_terminated g start (state_type := state_type) priorState)
+    (search_step : search_step_function g start)
+    (does_not_set_teriminate: search_step_does_not_terminate g start goal (state_type := state_type) search_step)
+    (termination_metric : state_type → ℕ × ℕ)
+    (decreasing_proof : ∀ s : state_type,
+        search_state_not_terminated g start (search_step goal s).1 → 
+        Prod.Lex (fun x1 x2 => x1 < x2) (fun x1 x2 => x1 < x2)
+        (termination_metric (search_step goal s).1) (termination_metric s)):
+    state_type × Bool :=
+  let qq := search_step goal priorState
+  let nextState := qq.fst
+  let result := qq.snd
+  if result_is_none : result = none then 
+    let still_not_terminated : (has_base_search_state.to_base_state nextState).terminated = false := by
+      apply does_not_set_teriminate
+      apply result_is_none
+
+    --let still_not_terminated : nextState.terminated = false := by
+    search_recurse g start goal nextState
+      still_not_terminated search_step does_not_set_teriminate termination_metric decreasing_proof
+  else ⟨ nextState, result.get (by apply Option.isSome_iff_ne_none.mpr ; exact result_is_none) ⟩ 
+termination_by termination_metric priorState
+decreasing_by
+  apply decreasing_proof
+  apply still_not_terminated
+
+
+
+lemma search_recurse_obtain_termination_property [FinEnum V] [DecidableEq E] [DecidableEq V]
+    (g: WeightedDiGraph V E) (start : V)
+    {state_type : Type} [has_base_search_state g start state_type]
+    (goal : V)
+    (priorState : state_type)
+    (not_terminated : search_state_not_terminated g start (state_type := state_type) priorState)
+    (search_step : search_step_function g start)
+    (does_not_set_teriminate: search_step_does_not_terminate g start goal (state_type := state_type) search_step)
+    (termination_metric : state_type → ℕ × ℕ)
+    (decreasing_proof : ∀ s : state_type,
+        search_state_not_terminated g start (search_step goal s).1 → 
+        Prod.Lex (fun x1 x2 => x1 < x2) (fun x1 x2 => x1 < x2)
+        (termination_metric (search_step goal s).1) (termination_metric s))
+    -- until here all necessary for calling the search_recurse
+    (terminated_with : Bool) -- recursion terminated with
+    (property_after_termination : state_type → Prop):
+      (∀ s : state_type, (search_step goal s).2 = some terminated_with → property_after_termination (search_step goal s).1)
+    → 
+      ((search_recurse g start goal priorState not_terminated search_step does_not_set_teriminate termination_metric decreasing_proof).2 = terminated_with → 
+      property_after_termination (search_recurse g start goal priorState not_terminated search_step does_not_set_teriminate termination_metric decreasing_proof).1):= by
+      intro step_termination_property
+      intro recursion_terminated_with
+      unfold search_recurse at recursion_terminated_with ⊢
+      simp_all
+      split
+      · next search_step_returned_none =>
+        -- recursive case
+        simp_all
+        apply search_recurse_obtain_termination_property g start goal
+        rotate_right
+        · use terminated_with -- recursion termiantes with same result
+        · apply step_termination_property
+        · apply recursion_terminated_with
+      · next h =>
+        simp_all
+        apply step_termination_property
+        apply Option.eq_some_iff_get_eq.mpr
+        simp_all
+        apply Option.isSome_iff_ne_none.mpr
+        exact h
+termination_by termination_metric priorState
+decreasing_by
+  next step_returned_none =>
+  apply decreasing_proof
+
+  let nextState : state_type := (search_step goal priorState).1
+  let still_not_terminated : (has_base_search_state.to_base_state nextState).terminated = false := by
+      apply does_not_set_teriminate
+      apply step_returned_none
+
+  apply still_not_terminated
+
+
+abbrev invar_carries_over_step [FinEnum V] [DecidableEq E] [DecidableEq V]
+    (g: WeightedDiGraph V E)(start : V)
+    {state_type : Type} [has_base_search_state g start state_type]
+    (goal : V)
+    (search_step : search_step_function g start (state_type := state_type))
+    (invar : state_type → Prop) :=
+      ∀ s : state_type, invar s → invar (search_step goal s).fst
+
+
+abbrev base_invar_carries_over_step [FinEnum V] [DecidableEq E] [DecidableEq V]
+    (g: WeightedDiGraph V E)(start : V)
+    {state_type : Type} [has_base_search_state g start state_type]
+    (goal : V)
+    (search_step : search_step_function g start (state_type := state_type))
+    (invar : base_search_state g start → Prop) :=
+      ∀ s : state_type, invar (has_base_search_state.to_base_state s) → invar (has_base_search_state.to_base_state (search_step goal s).fst)
+
+
+
+lemma search_recurse_lift_invariant [FinEnum V] [DecidableEq E] [DecidableEq V]
+    (g: WeightedDiGraph V E) (start : V)
+    {state_type : Type} [has_base_search_state g start state_type]
+    (goal : V)
+    (priorState : state_type)
+    (not_terminated : search_state_not_terminated g start (state_type := state_type) priorState)
+    (search_step : search_step_function g start)
+    (does_not_set_teriminate: search_step_does_not_terminate g start goal (state_type := state_type) search_step)
+    (termination_metric : state_type → ℕ × ℕ)
+    (decreasing_proof : ∀ s : state_type,
+        search_state_not_terminated g start (search_step goal s).1 → 
+        Prod.Lex (fun x1 x2 => x1 < x2) (fun x1 x2 => x1 < x2)
+        (termination_metric (search_step goal s).1) (termination_metric s))
+    -- until here all necessary for calling the search_recurse
+    (invar : state_type → Prop):
+      invar priorState ∧ (invar_carries_over_step g start goal search_step invar)
+         → invar (search_recurse g start goal priorState not_terminated search_step does_not_set_teriminate termination_metric decreasing_proof).fst:= by
+      intro ⟨ prior_invar, invar_carries ⟩ 
+      unfold search_recurse 
+      simp_all
+      split
+      · next search_step_returned_none =>
+        -- recursive case
+        apply search_recurse_lift_invariant g start goal
+        constructor
+        · unfold invar_carries_over_step at invar_carries
+          apply invar_carries
+          exact prior_invar
+        · exact invar_carries
+      · next h =>
+        simp_all
+termination_by termination_metric priorState
+decreasing_by
+  next step_returned_none =>
+  apply decreasing_proof
+
+  let nextState : state_type := (search_step goal priorState).1
+  let still_not_terminated : (has_base_search_state.to_base_state nextState).terminated = false := by
+      apply does_not_set_teriminate
+      apply step_returned_none
+
+  apply still_not_terminated
+
+
+lemma search_recurse_lift_base_invariant [FinEnum V] [DecidableEq E] [DecidableEq V]
+    (g: WeightedDiGraph V E) (start : V)
+    {state_type : Type} [has_base_search_state g start state_type]
+    (goal : V)
+    (priorState : state_type)
+    (not_terminated : search_state_not_terminated g start (state_type := state_type) priorState)
+    (search_step : search_step_function g start)
+    (does_not_set_teriminate: search_step_does_not_terminate g start goal (state_type := state_type) search_step)
+    (termination_metric : state_type → ℕ × ℕ)
+    (decreasing_proof : ∀ s : state_type,
+        search_state_not_terminated g start (search_step goal s).1 → 
+        Prod.Lex (fun x1 x2 => x1 < x2) (fun x1 x2 => x1 < x2)
+        (termination_metric (search_step goal s).1) (termination_metric s))
+    -- until here all necessary for calling the search_recurse
+    (invar : base_search_state g start → Prop):
+      invar (has_base_search_state.to_base_state priorState)
+      ∧ (base_invar_carries_over_step g start goal search_step invar)
+         → invar (has_base_search_state.to_base_state (search_recurse g start goal priorState not_terminated search_step does_not_set_teriminate termination_metric decreasing_proof).fst) := by
+      intro ⟨invar_holds_on_base, invar_carries⟩
+      apply search_recurse_lift_invariant g start goal priorState not_terminated search_step does_not_set_teriminate termination_metric decreasing_proof (fun x => invar (has_base_search_state.to_base_state x)) -- fun needed to tell lean what the "invariant" is it should apply
+      constructor
+      · use invar_holds_on_base
+      · use invar_carries
+
+
+--∀ goal : V, 
+--
+--    (dfs_recurse g start goal priorState not_terminated).2 = true →
+--     goal ∈ (dfs_recurse g start goal priorState not_terminated).1.visited := by
+--
+--    (dfs_recurse g start goal priorState not_terminated).2 = false
+--    → goal ∉ priorState.stack
+--
+--    (dfs_recurse g start goal priorState not_terminated).2 = false →
+--     (dfs_recurse g start goal priorState not_terminated).1.stack = [] := by
+--
+--    (dfs_recurse g start goal priorState not_terminated).2 = false 
+--    ∧ goal ∉ priorState.visited
+--    → goal ∉ (dfs_recurse g start goal priorState not_terminated).1.visited := by
